EffectSSA/ProofSketch/Notation/Reduce.lean
@@ -1,0 +1,67 @@
+module
+
+/-!
+# Reduction Semantics
+-/
+public section
+namespace EffectSSA.ProofSketch
+
+/-! ## Reduce Class -/
+
+class Reduce (α : Type) where
+  ReducesTo : α → α → Prop
+  /--
+  For now, we assume that small-step reduction is deterministic.
+  I'm not 100% sure we actually need this fact in the proof; it's here moreso
+  because I'm not convinced I'll get the subtleties of the *statement* of
+  contextual/denotational equivalence right in the presence of non-determinism.
+  -/
+  -- TODO: Eventually generalize this, and triple-check that the contextual and
+  --   denotational equivalence statements still make sense when we do.
+  eq_of_reducesTo_of_reducesTo : ∀ {x y z}, ReducesTo x y → ReducesTo x z → y = z := by grind
+
+export Reduce (ReducesTo)
+scoped infixl:50 " ⟹ " => ReducesTo
+
+/-! ## Transitive Closure -/
+section Closure
+
+/--
+`x ⟹+ y` holds when `x` reduces to `y` in one or more steps.
+
+That is, `⟹+` is the transitive closure of `⟹`.
+-/
+inductive TReducesTo {α} [Reduce α] : α → α → Prop where
+  | init {x y} : ReducesTo x y → TReducesTo x y
+  | step {x y z} : ReducesTo x y → TReducesTo y z → TReducesTo x z
+scoped infixl:arg " ⟹+ " => TReducesTo
+
+class BReduce (α : Type) (β : outParam Type) extends Reduce α where
+  /-- Type `β` can be seen as a subset of states in `α` which describe value. -/
+  stateOfValue : β → α
+  /-- Values ought to be terminal, i.e, may not reduce further. -/
+  terminal_value : ∀ (b : β) (y : α), ¬(stateOfValue b ⟹ y) := by grind
+
+@[grind] def BReducesTo {α β} [BReduce α β] : α → β → Prop :=
+  fun x y => x ⟹+ (BReduce.stateOfValue y)
+scoped infixl:50 " ⇓ " => BReducesTo
+
+namespace TReducesTo
+variable {α} [Reduce α] {x y z : α}
+
+attribute [grind ., grind →] init
+
+@[grind →] theorem trans : x ⟹+ y → y ⟹+ z → x ⟹+ z := by
+  intro h₁ h₂
+  induction h₁ <;> (
+    apply TReducesTo.step
+    · assumption
+    · grind
+  )
+
+instance : Trans (α:=α) (· ⟹+ ·) (· ⟹+ ·) (· ⟹+ ·) where trans := by grind
+instance : Trans (α:=α) (· ⟹+ ·) (· ⟹ ·) (· ⟹+ ·) where trans := by grind
+instance : Trans (α:=α) (· ⟹ ·) (· ⟹+ ·) (· ⟹+ ·) where trans := by grind
+
+end TReducesTo
+end Closure
